[Parikh] remove Pilling's lemma, rename a lot of stuff and add some documentation

Parikh/Eq_Sys.thy
@@ -1,19 +1,35 @@
 theory Eq_Sys
   imports
-    "./Lfun"
-    "./Parikh_Img"
+    "Lfun"
+    "Parikh_Img"
     "../CFG"
     "../CFL"
 begin
 
+(* TODO: remove unnecessary definitions and rename *)
+
+text \<open>In his proof, Pilling uses the fact that each CFG has an associated system of equations such
+that the CFG is the system's minimal solution. In this file, we will introduce for a given CFG two
+equation systems - one which assumes that the alphabet is commutative, i.e. only considers
+the languages' parikh images, and one which does not make this assumption - and show that the CFG
+is indeed the minimal solution of both.\<close>
+
+
 section \<open>systems of equations\<close>
 
-(* TODO: remove unused definitions, more consequent wording *)
+text \<open>Given an system of equations
+\<open>X\<^sub>0 \<supseteq> r\<^sub>0, X\<^sub>1 \<supseteq> r\<^sub>1, X\<^sub>2 \<supseteq> r\<^sub>2, \<dots>\<close> or \<open>\<Psi> X\<^sub>0 \<supseteq> \<Psi> r\<^sub>0, \<Psi> X\<^sub>1 \<supseteq> \<Psi> r\<^sub>1, \<Psi> X\<^sub>2 \<supseteq> \<Psi> r\<^sub>2, \<dots>\<close>
+(depending on the context), we represent it as a list of of language functions where we identify
+each of the variables \<open>X\<^sub>0, X\<^sub>1, X\<^sub>2, \<dots>\<close>, by its integer, i.e. \<open>Var i\<close> denotes the variable \<open>X\<^sub>i\<close>.
+The \<open>i\<close>-th item of the list then represents the right-hand side \<open>r\<^sub>i\<close> of the \<open>i\<close>-th equation.\<close>
 
-(* We just represent the right hand sides *)
-type_synonym 'a eq_sys = "'a lfun list"
+type_synonym 'a eq_sys = "'a rlexp list"
 
-(* solves equation with \<subseteq> *)
+
+subsection \<open>system of equations without Parikh images\<close>
+
+text \<open>Now we can define what it means for a valuation \<open>v\<close> to solve the classic system of equations,
+i.e. the one without Parikh images:\<close>
 definition solves_ineq_sys :: "'a eq_sys \<Rightarrow> 'a valuation \<Rightarrow> bool" where
   "solves_ineq_sys sys v \<equiv> \<forall>i < length sys. eval (sys ! i) v \<subseteq> v i"
 
@@ -21,33 +37,58 @@ definition solves_ineq_sys :: "'a eq_sys \<Rightarrow> 'a valuation \<Rightarrow
 definition solves_eq_sys :: "'a eq_sys \<Rightarrow> 'a valuation \<Rightarrow> bool" where
   "solves_eq_sys sys v \<equiv> \<forall>i < length sys. eval (sys ! i) v = v i"
 
+text \<open>\<open>sol\<close> is a minimal solution iff it is a solution and there is no smaller solution:\<close>
+definition min_sol_ineq_sys :: "'a eq_sys \<Rightarrow> 'a valuation \<Rightarrow> bool" where
+  "min_sol_ineq_sys sys sol \<equiv>
+    solves_ineq_sys sys sol \<and> (\<forall>sol'. solves_ineq_sys sys sol' \<longrightarrow> (\<forall>x. sol x \<subseteq> sol' x))"
+
+
+subsection \<open>System of equations with Parikh images\<close>
+
+text \<open>Now we look at the system of equations where the Parikh image is applied on both sides of
+each equation. First, we introduce what it means for a valuation \<open>v\<close> to solve the \<open>x\<close>-th equation:\<close>
 (* solves equation with \<subseteq>, only caring about the Parikh image *)
-definition solves_ineq_comm :: "nat \<Rightarrow> 'a lfun \<Rightarrow> 'a valuation \<Rightarrow> bool" where
+definition solves_ineq_comm :: "nat \<Rightarrow> 'a rlexp \<Rightarrow> 'a valuation \<Rightarrow> bool" where
   "solves_ineq_comm x eq v \<equiv> parikh_img (eval eq v) \<subseteq> parikh_img (v x)"
 
+text \<open>A valuation \<open>v\<close> solves the whole system iff it solves all equations:\<close>
 (* solves equation system with \<subseteq>, only caring about the Parikh image *)
 definition solves_ineq_sys_comm :: "'a eq_sys \<Rightarrow> 'a valuation \<Rightarrow> bool" where
   "solves_ineq_sys_comm sys v \<equiv> \<forall>i < length sys. solves_ineq_comm i (sys ! i) v"
 
 (* solves equation with =, only caring about the Parikh image*)
-definition solves_eq_comm :: "nat \<Rightarrow> 'a lfun \<Rightarrow> 'a valuation \<Rightarrow> bool" where
+definition solves_eq_comm :: "nat \<Rightarrow> 'a rlexp \<Rightarrow> 'a valuation \<Rightarrow> bool" where
   "solves_eq_comm x eq v \<equiv> parikh_img (eval eq v) = parikh_img (v x)"
 
 (* solves equation system with =, only caring about the Parikh image *)
 definition solves_eq_sys_comm :: "'a eq_sys \<Rightarrow> 'a valuation \<Rightarrow> bool" where
   "solves_eq_sys_comm sys v \<equiv> \<forall>i < length sys. solves_eq_comm i (sys ! i) v"
 
-(* Substituion into each equation of a system *)
-definition subst_sys :: "(nat \<Rightarrow> 'a lfun) \<Rightarrow> 'a eq_sys \<Rightarrow> 'a eq_sys" where
-  "subst_sys \<equiv> map \<circ> subst"
-
-definition partial_sol_ineq :: "nat \<Rightarrow> 'a lfun \<Rightarrow> 'a lfun \<Rightarrow> bool" where
+text \<open>We introduce partial solutions, i.e. solutions which might depend on one or multiple variables.
+They are therefore not represented as valuations, but as language functions (TODO). \<open>sol\<close> is a partial
+solution of the \<open>x\<close>-th equation iff it solves the equation independent on the values of the other
+variables, i.e. independent on the valuation as long as the valuation and \<open>sol\<close> coincide.
+Note that \<open>sol\<close> might depend on the variable \<open>x\<close> (we will deal with this problem later)\<close>
+definition partial_sol_ineq :: "nat \<Rightarrow> 'a rlexp \<Rightarrow> 'a rlexp \<Rightarrow> bool" where
   "partial_sol_ineq x eq sol \<equiv> \<forall>v. v x = eval sol v \<longrightarrow> solves_ineq_comm x eq v"
 
-definition solution_ineq_sys :: "'a eq_sys \<Rightarrow> (nat \<Rightarrow> 'a lfun) \<Rightarrow> bool" where
+text \<open>We generalize this to partial solutions of whole systems of equations:
+\<open>sols\<close> maps each variable \<open>i\<close> to a language function (TODO) representing the partial solution
+of the \<open>i\<close>-th equation (Note that \<open>sols\<close> is defined on all natural numbers, though).
+\<open>sols\<close> is a partial solution of the whole system iff all valuations coinciding with \<open>sols\<close> solve
+the system of equations:\<close>
+definition solution_ineq_sys :: "'a eq_sys \<Rightarrow> (nat \<Rightarrow> 'a rlexp) \<Rightarrow> bool" where
   "solution_ineq_sys sys sols \<equiv> \<forall>v. (\<forall>x. v x = eval (sols x) v) \<longrightarrow> solves_ineq_sys_comm sys v"
 
-definition partial_min_sol_ineq_sys :: "nat \<Rightarrow> 'a eq_sys \<Rightarrow> (nat \<Rightarrow> 'a lfun) \<Rightarrow> bool" where
+text \<open>Given a system of equations \<open>sys\<close>, \<open>sols\<close> is a minimal partial solution of the first \<open>n\<close>
+equations of the system iff the following conditions are satisfied:
+1. \<open>sols\<close> is a partial solution of the system's first \<open>n\<close> equations
+2. \<open>sols\<close> does not assign a proper partial solution to the remaining equations,
+   i.e. \<open>sols i = Var i\<close> for \<open>i \<ge> n\<close>
+3. No language function (TODO) in \<open>sols\<close> depends on variables smaller than \<open>n\<close>.
+   Furthermore, the partial solution of no equation depends on variables not occurring in the equation system
+4. There is no partial solution smaller than \<open>sols\<close> which solves all of the first \<open>n\<close> equations\<close>
+definition partial_min_sol_ineq_sys :: "nat \<Rightarrow> 'a eq_sys \<Rightarrow> (nat \<Rightarrow> 'a rlexp) \<Rightarrow> bool" where
   "partial_min_sol_ineq_sys n sys sols \<equiv>
     solution_ineq_sys (take n sys) sols \<and>
     (\<forall>i \<ge> n. sols i = Var i) \<and>
@@ -57,22 +98,30 @@ definition partial_min_sol_ineq_sys :: "nat \<Rightarrow> 'a eq_sys \<Rightarrow
                   \<longrightarrow> (\<forall>i. parikh_img (eval (sols i) v') \<subseteq> parikh_img (v' i)))"
 
 
-definition partial_min_sol_one_ineq :: "nat \<Rightarrow> 'a lfun \<Rightarrow> 'a lfun \<Rightarrow> bool" where
+text \<open>Given the \<open>x\<close>-th equation \<open>eq\<close>, \<open>sol\<close> is a minimal partial solution of this equation iff
+1. \<open>sol\<close> is a partial solution of \<open>eq\<close>,
+2. \<open>sol\<close> is a proper partial solution (i.e. it does not depend on \<open>x\<close>) and only depends on variables
+   occurring in the equation \<open>eq\<close> and
+3. no partial solution of the equation \<open>eq\<close> is smaller than \<open>sol\<close>\<close>
+definition partial_min_sol_one_ineq :: "nat \<Rightarrow> 'a rlexp \<Rightarrow> 'a rlexp \<Rightarrow> bool" where
   "partial_min_sol_one_ineq x eq sol \<equiv>
     partial_sol_ineq x eq sol \<and>
     vars sol \<subseteq> vars eq - {x} \<and>
     (\<forall>sol' v'. solves_ineq_comm x eq v' \<and> v' x = eval sol' v'
                \<longrightarrow> parikh_img (eval sol v') \<subseteq> parikh_img (v' x))"
 
-definition min_sol_ineq_sys :: "'a eq_sys \<Rightarrow> 'a valuation \<Rightarrow> bool" where
-  "min_sol_ineq_sys sys sol \<equiv>
-    solves_ineq_sys sys sol \<and> (\<forall>sol'. solves_ineq_sys sys sol' \<longrightarrow> (\<forall>x. sol x \<subseteq> sol' x))"
 
+text \<open>\<open>sol\<close> is a minimal solution of the system \<open>sys\<close> of equations iff it is a solution
+and there is no smaller solution:\<close>
 definition min_sol_ineq_sys_comm :: "'a eq_sys \<Rightarrow> 'a valuation \<Rightarrow> bool" where
   "min_sol_ineq_sys_comm sys sol \<equiv>
     solves_ineq_sys_comm sys sol \<and>
     (\<forall>sol'. solves_ineq_sys_comm sys sol' \<longrightarrow> (\<forall>x. parikh_img (sol x) \<subseteq> parikh_img (sol' x)))"
 
+
+text \<open>Substitution into each equation of a system:\<close>
+definition subst_sys :: "(nat \<Rightarrow> 'a rlexp) \<Rightarrow> 'a eq_sys \<Rightarrow> 'a eq_sys" where
+  "subst_sys \<equiv> map \<circ> subst"
 
 lemma subst_sys_subst:
   assumes "i < length sys"
@@ -80,6 +129,8 @@ lemma subst_sys_subst:
   unfolding subst_sys_def by (simp add: assms)
 
 
+text \<open>If the parikh image of two equations \<open>f\<close> and \<open>g\<close> is identical on all valuations, then their
+minimal partial solution is identical, too:\<close>
 lemma same_min_sol_if_same_parikh_img:
   assumes same_parikh_img: "\<forall>v. parikh_img (eval f v) = parikh_img (eval g v)"
       and same_vars:       "vars f - {x} = vars g - {x}"
@@ -98,7 +149,10 @@ qed
 
 
 
-section \<open>CFL as minimal solution of equation system\<close>
+section \<open>CFG as minimal solution of equation system\<close>
+
+text \<open>We show that each CFG induces a system of equations such that the CFG's language is the
+minimal solution of this system\<close>
 
 definition bij_Nt_Var :: "'n set \<Rightarrow> (nat \<Rightarrow> 'n) \<Rightarrow> ('n \<Rightarrow> nat) \<Rightarrow> bool" where
   "bij_Nt_Var A \<gamma> \<gamma>' \<equiv> bij_betw \<gamma> {..< card A} A \<and> bij_betw \<gamma>' A {..< card A}
@@ -117,14 +171,14 @@ proof -
 qed
 
 
-definition lfun_sym :: "('n \<Rightarrow> nat) \<Rightarrow> ('n, 't) sym \<Rightarrow> 't lfun" where
-  "lfun_sym \<gamma>' s = (case s of Tm a \<Rightarrow> Const {[a]} | Nt A \<Rightarrow> Var (\<gamma>' A))"
+definition rlexp_sym :: "('n \<Rightarrow> nat) \<Rightarrow> ('n, 't) sym \<Rightarrow> 't rlexp" where
+  "rlexp_sym \<gamma>' s = (case s of Tm a \<Rightarrow> Const {[a]} | Nt A \<Rightarrow> Var (\<gamma>' A))"
 
-definition lfun_concats :: "'a lfun list \<Rightarrow> 'a lfun" where
-  "lfun_concats fs = foldr Concat fs (Const {[]})"
+definition rlexp_concats :: "'a rlexp list \<Rightarrow> 'a rlexp" where
+  "rlexp_concats fs = foldr Concat fs (Const {[]})"
 
-definition lfun_syms :: "('n \<Rightarrow> nat) \<Rightarrow> ('n, 't) syms \<Rightarrow> 't lfun" where
-  "lfun_syms \<gamma>' w = lfun_concats (map (lfun_sym \<gamma>') w)"
+definition rlexp_syms :: "('n \<Rightarrow> nat) \<Rightarrow> ('n, 't) syms \<Rightarrow> 't rlexp" where
+  "rlexp_syms \<gamma>' w = rlexp_concats (map (rlexp_sym \<gamma>') w)"
 
 
 (* Some auxiliary lemmas *)
@@ -156,113 +210,113 @@ begin
 
 abbreviation "CFG_sys sys \<equiv>
   length sys = card (Nts P) \<and>
-    (\<forall>i < card (Nts P). regular_fun (sys ! i) \<and> (\<forall>x \<in> vars (sys ! i). x < card (Nts P))
+    (\<forall>i < card (Nts P). reg_eval (sys ! i) \<and> (\<forall>x \<in> vars (sys ! i). x < card (Nts P))
                         \<and> (\<forall>s L. (\<forall>A \<in> Nts P. s (\<gamma>' A) = L A)
                             \<longrightarrow> eval (sys ! i) s = subst_lang P L (\<gamma> i)))"
 
 abbreviation "sol \<equiv> \<lambda>i. if i < card (Nts P) then Lang_lfp P (\<gamma> i) else {}"
 
-lemma lfun_sym_reg: "regular_fun (lfun_sym \<gamma>' s)"
-unfolding lfun_sym_def proof (induction s)
+lemma rlexp_sym_reg: "reg_eval (rlexp_sym \<gamma>' s)"
+unfolding rlexp_sym_def proof (induction s)
   case (Tm x)
   have "regular_lang {[x]}" by (meson lang.simps(3))
   then show ?case by auto
 qed auto
 
-lemma lfun_concats_reg:
-  assumes "\<forall>f \<in> set fs. regular_fun f"
-    shows "regular_fun (lfun_concats fs)"
-  using assms epsilon_regular unfolding lfun_concats_def by (induction fs) auto
+lemma rlexp_concats_reg:
+  assumes "\<forall>f \<in> set fs. reg_eval f"
+    shows "reg_eval (rlexp_concats fs)"
+  using assms epsilon_regular unfolding rlexp_concats_def by (induction fs) auto
 
-lemma lfun_syms_reg: "regular_fun (lfun_syms \<gamma>' w)"
+lemma rlexp_syms_reg: "reg_eval (rlexp_syms \<gamma>' w)"
 proof -
-  from lfun_sym_reg have "\<forall>s \<in> set w. regular_fun (lfun_sym \<gamma>' s)" by blast
-  with lfun_concats_reg show ?thesis unfolding lfun_syms_def
+  from rlexp_sym_reg have "\<forall>s \<in> set w. reg_eval (rlexp_sym \<gamma>' s)" by blast
+  with rlexp_concats_reg show ?thesis unfolding rlexp_syms_def
     by (metis (no_types, lifting) image_iff list.set_map)
 qed
 
 
-lemma lfun_sym_vars_Nt:
+lemma rlexp_sym_vars_Nt:
   assumes "s (\<gamma>' A) = L A"
-    shows "vars (lfun_sym \<gamma>' (Nt A)) = {\<gamma>' A}"
-  using assms unfolding lfun_sym_def by simp
+    shows "vars (rlexp_sym \<gamma>' (Nt A)) = {\<gamma>' A}"
+  using assms unfolding rlexp_sym_def by simp
 
-lemma lfun_sym_vars_Tm: "vars (lfun_sym \<gamma>' (Tm x)) = {}"
-  unfolding lfun_sym_def by simp
+lemma rlexp_sym_vars_Tm: "vars (rlexp_sym \<gamma>' (Tm x)) = {}"
+  unfolding rlexp_sym_def by simp
 
-lemma lfun_concats_vars: "vars (lfun_concats fs) = \<Union>(vars ` set fs)"
-  unfolding lfun_concats_def by (induction fs) simp_all
+lemma rlexp_concats_vars: "vars (rlexp_concats fs) = \<Union>(vars ` set fs)"
+  unfolding rlexp_concats_def by (induction fs) simp_all
 
 (* it even holds equality, but we will not need it *)
-lemma insts'_vars: "vars (lfun_syms \<gamma>' w) \<subseteq> \<gamma>' ` nts_syms w"
+lemma insts'_vars: "vars (rlexp_syms \<gamma>' w) \<subseteq> \<gamma>' ` nts_syms w"
 proof
   fix x
-  assume "x \<in> vars (lfun_syms \<gamma>' w)"
-  with lfun_concats_vars have "x \<in> \<Union>(vars ` set (map (lfun_sym \<gamma>') w))"
-    unfolding lfun_syms_def by blast
-  then obtain f where *: "f \<in> set (map (lfun_sym \<gamma>') w) \<and> x \<in> vars f" by blast
-  then obtain s where **: "s \<in> set w \<and> lfun_sym \<gamma>' s = f" by auto
-  with * lfun_sym_vars_Tm obtain A where ***: "s = Nt A" by (metis empty_iff sym.exhaust)
+  assume "x \<in> vars (rlexp_syms \<gamma>' w)"
+  with rlexp_concats_vars have "x \<in> \<Union>(vars ` set (map (rlexp_sym \<gamma>') w))"
+    unfolding rlexp_syms_def by blast
+  then obtain f where *: "f \<in> set (map (rlexp_sym \<gamma>') w) \<and> x \<in> vars f" by blast
+  then obtain s where **: "s \<in> set w \<and> rlexp_sym \<gamma>' s = f" by auto
+  with * rlexp_sym_vars_Tm obtain A where ***: "s = Nt A" by (metis empty_iff sym.exhaust)
   with ** have ****: "A \<in> nts_syms w" unfolding nts_syms_def by blast
-  with lfun_sym_vars_Nt have "vars (lfun_sym \<gamma>' (Nt A)) = {\<gamma>' A}" by blast
+  with rlexp_sym_vars_Nt have "vars (rlexp_sym \<gamma>' (Nt A)) = {\<gamma>' A}" by blast
   with * ** *** **** show "x \<in> \<gamma>' ` nts_syms w" by blast
 qed
 
 
-lemma lfun_sym_inst_Nt:
+lemma rlexp_sym_inst_Nt:
   assumes "v (\<gamma>' A) = L A"
-    shows "eval (lfun_sym \<gamma>' (Nt A)) v = inst_sym L (Nt A)"
-  using assms unfolding lfun_sym_def inst_sym_def by force
+    shows "eval (rlexp_sym \<gamma>' (Nt A)) v = inst_sym L (Nt A)"
+  using assms unfolding rlexp_sym_def inst_sym_def by force
 
-lemma lfun_sym_inst_Tm: "eval (lfun_sym \<gamma>' (Tm a)) v = inst_sym L (Tm a)"
-  unfolding lfun_sym_def inst_sym_def by force
+lemma rlexp_sym_inst_Tm: "eval (rlexp_sym \<gamma>' (Tm a)) v = inst_sym L (Tm a)"
+  unfolding rlexp_sym_def inst_sym_def by force
 
-lemma lfun_concats_concats:
+lemma rlexp_concats_concats:
   assumes "length fs = length Ls"
       and "\<forall>i < length fs. eval (fs ! i) v = Ls ! i"
-    shows "eval (lfun_concats fs) v = concats Ls"
+    shows "eval (rlexp_concats fs) v = concats Ls"
 using assms proof (induction fs arbitrary: Ls)
   case Nil
-  then show ?case unfolding lfun_concats_def concats_def by simp
+  then show ?case unfolding rlexp_concats_def concats_def by simp
 next
   case (Cons f1 fs)
   then obtain L1 Lr where *: "Ls = L1#Lr" by (metis length_Suc_conv)
-  with Cons have "eval (lfun_concats fs) v = concats Lr" by fastforce
+  with Cons have "eval (rlexp_concats fs) v = concats Lr" by fastforce
   moreover from Cons.prems * have "eval f1 v = L1" by force
-  ultimately show ?case unfolding lfun_concats_def concats_def by (simp add: "*")
+  ultimately show ?case unfolding rlexp_concats_def concats_def by (simp add: "*")
 qed
 
-lemma lfun_syms_insts:
+lemma rlexp_syms_insts:
   assumes "\<forall>A \<in> nts_syms w. v (\<gamma>' A) = L A"
-    shows "eval (lfun_syms \<gamma>' w) v = inst_syms L w"
+    shows "eval (rlexp_syms \<gamma>' w) v = inst_syms L w"
 proof -
-  have "\<forall>i < length w. eval (lfun_sym \<gamma>' (w!i)) v = inst_sym L (w!i)"
+  have "\<forall>i < length w. eval (rlexp_sym \<gamma>' (w!i)) v = inst_sym L (w!i)"
   proof (rule allI, rule impI)
     fix i
     assume "i < length w"
-    then show "eval (lfun_sym \<gamma>' (w ! i)) v = inst_sym L (w ! i)"
+    then show "eval (rlexp_sym \<gamma>' (w ! i)) v = inst_sym L (w ! i)"
       using assms proof (induction "w!i")
       case (Nt A)
       then have "v (\<gamma>' A) = L A" unfolding nts_syms_def by force
-      with lfun_sym_inst_Nt Nt show ?case by metis
+      with rlexp_sym_inst_Nt Nt show ?case by metis
     next
       case (Tm x)
-      with lfun_sym_inst_Tm show ?case by metis
+      with rlexp_sym_inst_Tm show ?case by metis
     qed
   qed
-  then show ?thesis unfolding lfun_syms_def inst_syms_def using lfun_concats_concats
+  then show ?thesis unfolding rlexp_syms_def inst_syms_def using rlexp_concats_concats
     by (metis (mono_tags, lifting) length_map nth_map)
 qed
 
 
-lemma subst_lang_lfun:
-  "\<exists>eq. regular_fun eq \<and> vars eq \<subseteq> \<gamma>' ` Nts P
+lemma subst_lang_rlexp:
+  "\<exists>eq. reg_eval eq \<and> vars eq \<subseteq> \<gamma>' ` Nts P
          \<and> (\<forall>v L. (\<forall>A \<in> Nts P. v (\<gamma>' A) = L A) \<longrightarrow> eval eq v = subst_lang P L A)"
 proof -
-  let ?Insts = "(lfun_syms \<gamma>') ` (Rhss P A)"
+  let ?Insts = "(rlexp_syms \<gamma>') ` (Rhss P A)"
   from finite_Rhss[OF finite_P] have "finite ?Insts" by simp
-  moreover from lfun_syms_reg have "\<forall>f \<in> ?Insts. regular_fun f" by blast
-  ultimately obtain eq where *: "regular_fun eq \<and> \<Union>(vars ` ?Insts) = vars eq
+  moreover from rlexp_syms_reg have "\<forall>f \<in> ?Insts. reg_eval f" by blast
+  ultimately obtain eq where *: "reg_eval eq \<and> \<Union>(vars ` ?Insts) = vars eq
                                   \<and> (\<forall>v. (\<Union>f \<in> ?Insts. eval f v) = eval eq v)"
     using finite_Union_regular by metis
 
@@ -271,7 +325,7 @@ proof -
     fix x
     assume "x \<in> vars eq"
     with * obtain f where **: "f \<in> ?Insts \<and> x \<in> vars f" by blast
-    then obtain w where ***: "w \<in> Rhss P A \<and> f = lfun_syms \<gamma>' w" by blast
+    then obtain w where ***: "w \<in> Rhss P A \<and> f = rlexp_syms \<gamma>' w" by blast
     with ** insts'_vars have "x \<in> \<gamma>' ` nts_syms w" by auto
     with *** show "x \<in> \<gamma>' ` Nts P" unfolding Nts_def Rhss_def by blast
   qed
@@ -281,12 +335,12 @@ proof -
     fix v :: "nat \<Rightarrow> 'a lang" and L :: "'n \<Rightarrow> 'a lang"
     assume state_L: "\<forall>A \<in> Nts P. v (\<gamma>' A) = L A"
 
-    have "\<forall>w \<in> Rhss P A. eval (lfun_syms \<gamma>' w) v = inst_syms L w"
+    have "\<forall>w \<in> Rhss P A. eval (rlexp_syms \<gamma>' w) v = inst_syms L w"
     proof
       fix w
       assume "w \<in> Rhss P A"
       with state_L Nts_nts_syms have "\<forall>A \<in> nts_syms w. v (\<gamma>' A) = L A" by fast
-      from lfun_syms_insts[OF this] show "eval (lfun_syms \<gamma>' w) v = inst_syms L w" by blast
+      from rlexp_syms_insts[OF this] show "eval (rlexp_syms \<gamma>' w) v = inst_syms L w" by blast
     qed
 
     then have "subst_lang P L A = (\<Union>f \<in> ?Insts. eval f v)" unfolding subst_lang_def by auto
@@ -301,13 +355,13 @@ lemma CFG_as_eq_sys: "\<exists>sys. CFG_sys sys"
 proof -
   from bij_\<gamma>_\<gamma>' have *: "\<And>eq. vars eq \<subseteq> \<gamma>' ` Nts P \<Longrightarrow> \<forall>x \<in> vars eq. x < card (Nts P)"
     unfolding bij_Nt_Var_def bij_betw_def by auto
-  from subst_lang_lfun have "\<forall>A. \<exists>eq. regular_fun eq \<and> vars eq \<subseteq> \<gamma>' ` Nts P \<and>
+  from subst_lang_rlexp have "\<forall>A. \<exists>eq. reg_eval eq \<and> vars eq \<subseteq> \<gamma>' ` Nts P \<and>
                              (\<forall>s L. (\<forall>A \<in> Nts P. s (\<gamma>' A) = L A) \<longrightarrow> eval eq s = subst_lang P L A)"
     by blast
-  with bij_\<gamma>_\<gamma>' * have "\<forall>i < card (Nts P). \<exists>eq. regular_fun eq \<and> (\<forall>x \<in> vars eq. x < card (Nts P))
+  with bij_\<gamma>_\<gamma>' * have "\<forall>i < card (Nts P). \<exists>eq. reg_eval eq \<and> (\<forall>x \<in> vars eq. x < card (Nts P))
                     \<and> (\<forall>s L. (\<forall>A \<in> Nts P. s (\<gamma>' A) = L A) \<longrightarrow> eval eq s = subst_lang P L (\<gamma> i))"
     unfolding bij_Nt_Var_def by metis
-  with Skolem_list_nth[where P="\<lambda>i eq. regular_fun eq \<and> (\<forall>x \<in> vars eq. x < card (Nts P))
+  with Skolem_list_nth[where P="\<lambda>i eq. reg_eval eq \<and> (\<forall>x \<in> vars eq. x < card (Nts P))
                        \<and> (\<forall>s L. (\<forall>A \<in> Nts P. s (\<gamma>' A) = L A) \<longrightarrow> eval eq s = subst_lang P L (\<gamma> i))"]
     show ?thesis by blast
 qed
@@ -372,12 +426,12 @@ next
 qed
 
 lemma CFL_is_min_sol:
-  "\<exists>sys. (\<forall>eq \<in> set sys. regular_fun eq) \<and> (\<forall>eq \<in> set sys. \<forall>x \<in> vars eq. x < length sys)
+  "\<exists>sys. (\<forall>eq \<in> set sys. reg_eval eq) \<and> (\<forall>eq \<in> set sys. \<forall>x \<in> vars eq. x < length sys)
           \<and> min_sol_ineq_sys sys sol"
 proof -
   from CFG_as_eq_sys obtain sys where *: "CFG_sys sys" by blast
   then have "length sys = card (Nts P)" by blast
-  moreover from * have "\<forall>eq \<in> set sys. regular_fun eq" by (simp add: all_set_conv_all_nth)
+  moreover from * have "\<forall>eq \<in> set sys. reg_eval eq" by (simp add: all_set_conv_all_nth)
   moreover from * \<open>length sys = card (Nts P)\<close> have "\<forall>eq \<in> set sys. \<forall>x \<in> vars eq. x < length sys"
     by (simp add: all_set_conv_all_nth)
   moreover from CFG_sys_CFL_is_sol[OF *] CFG_sys_CFL_is_min[OF *]
@@ -388,8 +442,10 @@ qed
 end
 
 
-section \<open>Relationship between equation system with and without commutivity\<close>
+section \<open>Relationship between the system of equations with and the one without Parikh images\<close>
 
+text \<open>To any solution \<open>sol\<close> of a commutative system of equations, there corresponds
+a solution to the same non-commutative system which has the same Parikh image as \<open>sol\<close>\<close>
 lemma sol_comm_sol:
   assumes sol_is_sol_comm: "solves_ineq_sys_comm sys sol"
   shows   "\<exists>sol'. (\<forall>x. parikh_img (sol x) = parikh_img (sol' x)) \<and> solves_ineq_sys sys sol'"
@@ -406,7 +462,7 @@ proof
     with sol_is_sol_comm have "parikh_img (eval (sys ! i) sol) \<subseteq> parikh_img (sol i)"
       unfolding solves_ineq_sys_comm_def solves_ineq_comm_def by blast
     moreover from sol'_sol have "parikh_img (eval (sys ! i) ?sol') = parikh_img (eval (sys ! i) sol)"
-      using lfun_mono_parikh_eq by meson
+      using rlexp_mono_parikh_eq by meson
     ultimately have "parikh_img (eval (sys ! i) ?sol') \<subseteq> parikh_img (sol i)" by simp
     then show "eval (sys ! i) ?sol' \<subseteq> ?sol' i" using subseteq_comm_subseteq by metis
   qed
@@ -415,7 +471,8 @@ proof
     by simp
 qed
 
-
+text \<open>A minimal solution of the non-commutative system of equations is a solution of the
+commutative system of equations, as well.\<close>
 lemma min_sol_min_sol_comm:
   assumes "min_sol_ineq_sys sys sol"
     shows "min_sol_ineq_sys_comm sys sol"
@@ -436,7 +493,7 @@ unfolding min_sol_ineq_sys_comm_def proof
   qed
 qed
 
-
+text \<open>All minimal solutions of a commutative system of equations have the same Parikh image\<close>
 lemma min_sol_comm_unique:
   assumes sol1_is_min_sol: "min_sol_ineq_sys_comm sys sol1"
       and sol2_is_min_sol: "min_sol_ineq_sys_comm sys sol2"
