Parikh/Lfun.thy
@@ -5,57 +5,51 @@ theory Lfun
 begin
 
 
-section \<open>Definition of language functions\<close>
+section \<open>Definition of regular language expressions\<close>
 
-(* "language functions" are functions which get languages as arguments and also
-   produce languages.
-*)
+text \<open>Regular language expressions\<close>
+datatype 'a rlexp = Var nat                          (* Variable *)
+                  | Const "'a lang"                  (* Constant *)
+                  | Union "'a rlexp" "'a rlexp"
+                  | Concat "'a rlexp" "'a rlexp"     (* Concatenation *)
+                  | Star "'a rlexp"                  (* Kleene star*)
 
-datatype 'a lfun = Var nat                        (* Variable *)
-                 | Const "'a lang"                  (* Constant *)
-                 | Union2 "'a lfun" "'a lfun"
-                 | UnionC "nat \<Rightarrow> 'a lfun"      (* Countable union *)
-                 | Concat "'a lfun" "'a lfun"     (* Concatenation *)
-                 | Star "'a lfun"
 
-(* instantiate each variable with a language *)
+text \<open>instantiate each variable with a language\<close>
 type_synonym 'a valuation = "nat \<Rightarrow> 'a lang"
 
-(* evaluate function for a given state, this produces a language *)
-primrec eval :: "'a lfun \<Rightarrow> 'a valuation \<Rightarrow> 'a lang" where
+text \<open>evaluate the regular language expression for a given valuation, yielding a language\<close>
+primrec eval :: "'a rlexp \<Rightarrow> 'a valuation \<Rightarrow> 'a lang" where
   "eval (Var n) v = v n" |
   "eval (Const l) _ = l" |
-  "eval (Union2 f g) v = eval f v \<union> eval g v" |
-  "eval (UnionC f) v = (\<Union>i. eval (f i) v)" |
+  "eval (Union f g) v = eval f v \<union> eval g v" |
   "eval (Concat f g) v = eval f v @@ eval g v" |
   "eval (Star f) v = star (eval f v)"
 
-(* all variables occurring in a function *)
-primrec vars :: "'a lfun \<Rightarrow> nat set" where
+text \<open>all variables occurring in the regular language expression\<close>
+primrec vars :: "'a rlexp \<Rightarrow> nat set" where
   "vars (Var n) = {n}" |
   "vars (Const _) = {}" |
-  "vars (Union2 f g) = vars f \<union> vars g" |
-  "vars (UnionC f) = (\<Union>i. vars (f i))" |
+  "vars (Union f g) = vars f \<union> vars g" |
   "vars (Concat f g) = vars f \<union> vars g" |
   "vars (Star f) = vars f"
 
-(* substitute each occurrence of a variable i by the language function s i *)
-primrec subst :: "(nat \<Rightarrow> 'a lfun) \<Rightarrow> 'a lfun \<Rightarrow> 'a lfun" where
+text \<open>substitute each occurrence of a variable \<open>i\<close> by the regular language expression \<open>s i\<close>\<close>
+primrec subst :: "(nat \<Rightarrow> 'a rlexp) \<Rightarrow> 'a rlexp \<Rightarrow> 'a rlexp" where
   "subst s (Var n) = s n" |
   "subst _ (Const l) = Const l" |
-  "subst s (Union2 f g) = Union2 (subst s f) (subst s g)" |
-  "subst s (UnionC f) = UnionC (\<lambda>i. subst s (f i))" |
+  "subst s (Union f g) = Union (subst s f) (subst s g)" |
   "subst s (Concat f g) = Concat (subst s f) (subst s g)" |
   "subst s (Star f) = Star (subst s f)"
 
 
 
-section \<open>Some lemmas about the introduced functions\<close>
+section \<open>Some lemmas about regular language expressions\<close>
 
 lemma substitution_lemma:
   assumes "\<forall>i. v' i = eval (upd i) v"
   shows "eval (subst upd f) v = eval f v'"
-  using assms by (induction rule: lfun.induct) auto
+  using assms by (induction rule: rlexp.induct) auto
 
 lemma substitution_lemma_update:
   "eval (subst (Var(x := f')) f) v = eval f (v(x := eval f' v))"
@@ -126,34 +120,35 @@ qed
 
 
 
-section \<open>Monotonicity of language functions\<close>
+section \<open>Monotonicity of regular language expressions\<close>
 
-lemma lfun_mono_aux:
+lemma rlexp_mono_aux:
   assumes "\<forall>i \<in> vars f. v i \<subseteq> v' i"
   shows "eval f v \<subseteq> eval f v'"
-using assms proof (induction rule: lfun.induct)
+using assms proof (induction rule: rlexp.induct)
   case (Star x)
   then show ?case
-    by (smt (verit, best) eval.simps(6) in_star_iff_concat order_trans subsetI vars.simps(6))
+    by (smt (verit, best) eval.simps(5) in_star_iff_concat order_trans subsetI vars.simps(5))
 qed fastforce+
 
-lemma lfun_mono:
-  fixes f :: "'a lfun"
+text \<open>The actually monotonicity lemma\<close>
+lemma rlexp_mono:
+  fixes f :: "'a rlexp"
   shows "mono (eval f)"
-  using lfun_mono_aux by (metis le_funD monoI)
+  using rlexp_mono_aux by (metis le_funD monoI)
 
 
 
-section \<open>Continuity of language functions\<close>
+section \<open>Continuity of regular language expressions\<close>
 
-(* Surprisingly, I could not find such a lemma in Regular_Set.thy *)
 lemma langpow_mono:
   fixes A :: "'a lang"
   assumes "A \<subseteq> B"
   shows "A ^^ n \<subseteq> B ^^ n"
 using assms conc_mono[of A B] by (induction n) auto
 
-lemma lfun_cont_aux1:
+text \<open>The one direction:\<close>
+lemma rlexp_cont_aux1:
   assumes "\<forall>i. v i \<le> v (Suc i)"
       and "w \<in> (\<Union>i. eval f (v i))"
     shows "w \<in> eval f (\<lambda>x. \<Union>i. v i x)"
@@ -161,7 +156,7 @@ proof -
   from assms(2) obtain n where n_intro: "w \<in> eval f (v n)" by auto
   have "v n x \<subseteq> (\<Union>i. v i x)" for x by auto
   with n_intro show "?thesis"
-    using lfun_mono_aux[where v="v n" and v'="\<lambda>x. \<Union>i. v i x"] by auto
+    using rlexp_mono_aux[where v="v n" and v'="\<lambda>x. \<Union>i. v i x"] by auto
 qed
 
 lemma langpow_Union_eval:
@@ -178,85 +173,88 @@ next
   with Suc have "u \<in> (\<Union>i. eval f (v i)) \<and> u' \<in> (\<Union>i. eval f (v i) ^^ n)" by auto
   then obtain i j where i_intro: "u \<in> eval f (v i)" and j_intro: "u' \<in> eval f (v j) ^^ n" by blast
   let ?m = "max i j"
-  from i_intro Suc.prems(1) lfun_mono_aux have 1: "u \<in> eval f (v ?m)"
+  from i_intro Suc.prems(1) rlexp_mono_aux have 1: "u \<in> eval f (v ?m)"
     by (metis le_fun_def lift_Suc_mono_le max.cobounded1 subset_eq)
-  from Suc.prems(1) lfun_mono_aux have "eval f (v j) \<subseteq> eval f (v ?m)"
+  from Suc.prems(1) rlexp_mono_aux have "eval f (v j) \<subseteq> eval f (v ?m)"
     by (metis le_fun_def lift_Suc_mono_le max.cobounded2)
   with j_intro langpow_mono have 2: "u' \<in> eval f (v ?m) ^^ n" by auto
   from 1 2 show ?case using w_decomp by auto
 qed
 
-lemma lfun_cont_aux2:
+text \<open>The other direction:\<close>
+lemma rlexp_cont_aux2:
   assumes "\<forall>i. v i \<le> v (Suc i)"
       and "w \<in> eval f (\<lambda>x. \<Union>i. v i x)"
     shows "w \<in> (\<Union>i. eval f (v i))"
-using assms proof (induction arbitrary: w rule: lfun.induct)
+using assms proof (induction arbitrary: w rule: rlexp.induct)
   case (Concat f g)
   then obtain u u' where w_decomp: "w = u@u'"
     and "u \<in> eval f (\<lambda>x. \<Union>i. v i x) \<and> u' \<in> eval g (\<lambda>x. \<Union>i. v i x)" by auto
   with Concat have "u \<in> (\<Union>i. eval f (v i)) \<and> u' \<in> (\<Union>i. eval g (v i))" by auto
   then obtain i j where i_intro: "u \<in> eval f (v i)" and j_intro: "u' \<in> eval g (v j)" by blast
   let ?m = "max i j"
-  from i_intro Concat.prems(1) lfun_mono_aux have "u \<in> eval f (v ?m)"
+  from i_intro Concat.prems(1) rlexp_mono_aux have "u \<in> eval f (v ?m)"
     by (metis le_fun_def lift_Suc_mono_le max.cobounded1 subset_eq)
-  moreover from j_intro Concat.prems(1) lfun_mono_aux have "u' \<in> eval g (v ?m)"
+  moreover from j_intro Concat.prems(1) rlexp_mono_aux have "u' \<in> eval g (v ?m)"
     by (metis le_fun_def lift_Suc_mono_le max.cobounded2 subset_eq)
   ultimately show ?case using w_decomp by auto
 next
   case (Star f)
   then obtain n where n_intro: "w \<in> (eval f (\<lambda>x. \<Union>i. v i x)) ^^ n"
-    using eval.simps(6) star_pow by blast
+    using eval.simps(5) star_pow by blast
   with Star have "w \<in> (\<Union>i. eval f (v i)) ^^ n" using langpow_mono by blast
   with Star.prems have "w \<in> (\<Union>i. eval f (v i) ^^ n)" using langpow_Union_eval by auto
   then show ?case by (auto simp add: star_def)
 qed fastforce+
 
 
-(* The actual continuity lemma *)
-lemma lfun_cont:
+text \<open>The actual continuity lemma:\<close>
+lemma rlexp_cont:
   assumes "\<forall>i. v i \<le> v (Suc i)"
   shows "eval f (\<lambda>x. \<Union>i. v i x) = (\<Union>i. eval f (v i))"
 proof
-  from assms show "eval f (\<lambda>x. \<Union>i. v i x) \<subseteq> (\<Union>i. eval f (v i))" using lfun_cont_aux2 by auto
-  from assms show "(\<Union>i. eval f (v i)) \<subseteq> eval f (\<lambda>x. \<Union>i. v i x)" using lfun_cont_aux1 by blast
+  from assms show "eval f (\<lambda>x. \<Union>i. v i x) \<subseteq> (\<Union>i. eval f (v i))" using rlexp_cont_aux2 by auto
+  from assms show "(\<Union>i. eval f (v i)) \<subseteq> eval f (\<lambda>x. \<Union>i. v i x)" using rlexp_cont_aux1 by blast
 qed
 
 
 
-section \<open>Regular functions\<close>
+section \<open>Regular language expressions which evaluate to regular languages\<close>
 
-(* A regular function is a function which evaluates to a regular language
-   if all of its arguments are regular. This applies to all operations
-   defined for lfun, except the countable union (which is needed for the
-   proof of the lemma in Pilling's paper)
-*)
+text \<open>Evaluating regular language expressions can yield non-regular languages even if
+the valuation maps each variable to a regular language. This is because \<open>Const\<close> may introduce
+non-regular languages.
+We therefore introduce the predicate \<open>reg_eval\<close> which guarantees that a regular language expression
+\<open>f\<close> yields a regular language if the valuation maps all variables occurring in \<open>f\<close> to some regular
+language. This is achieved by only allowing regular languages as constants.
+However, note that \<open>reg_eval\<close> is an under-approximation, i.e. there exist regular language
+expressions which do not satisfy this predicate but evaluate to regular languages anyway.\<close>
 
-fun regular_fun :: "'a lfun \<Rightarrow> bool" where
-  "regular_fun (Var _) \<longleftrightarrow> True" |
-  "regular_fun (Const l) \<longleftrightarrow> regular_lang l" |
-  "regular_fun (Union2 f g) \<longleftrightarrow> regular_fun f \<and> regular_fun g" |
-  "regular_fun (Concat f g) \<longleftrightarrow> regular_fun f \<and> regular_fun g" |
-  "regular_fun (Star f) \<longleftrightarrow> regular_fun f" |
-  (* Might actually be a regular_fun, but in general it is not *)
-  "regular_fun (UnionC _) \<longleftrightarrow> False"
-
-
-lemma emptyset_regular: "regular_fun (Const {})"
-  using lang.simps(1) regular_fun.simps(2) by blast
-
-lemma epsilon_regular: "regular_fun (Const {[]})"
-  using lang.simps(2) regular_fun.simps(2) by blast
+fun reg_eval :: "'a rlexp \<Rightarrow> bool" where
+  "reg_eval (Var _) \<longleftrightarrow> True" |
+  "reg_eval (Const l) \<longleftrightarrow> regular_lang l" |
+  "reg_eval (Union f g) \<longleftrightarrow> reg_eval f \<and> reg_eval g" |
+  "reg_eval (Concat f g) \<longleftrightarrow> reg_eval f \<and> reg_eval g" |
+  "reg_eval (Star f) \<longleftrightarrow> reg_eval f"
 
 
-(* If all arguments are regular, a regular function evaluates to a regular language *)
-lemma regular_fun_regular:
-  assumes "regular_fun f"
+lemma emptyset_regular: "reg_eval (Const {})"
+  using lang.simps(1) reg_eval.simps(2) by blast
+
+lemma epsilon_regular: "reg_eval (Const {[]})"
+  using lang.simps(2) reg_eval.simps(2) by blast
+
+
+text \<open>If the valuation \<open>v\<close> maps all variables occurring in the regular language function \<open>f\<close> to
+some regular language, then evaluating \<open>f\<close> again yields a regular language.\<close>
+lemma reg_eval_regular:
+  assumes "reg_eval f"
       and "\<And>n. n \<in> vars f \<Longrightarrow> regular_lang (v n)"
     shows "regular_lang (eval f v)"
-using assms proof (induction rule: regular_fun.induct)
+using assms proof (induction rule: reg_eval.induct)
   case (3 f g)
   then obtain r1 r2 where "Regular_Exp.lang r1 = eval f v \<and> Regular_Exp.lang r2 = eval g v" by auto
-  then have "Regular_Exp.lang (Plus r1 r2) = eval (Union2 f g) v" by simp
+  then have "Regular_Exp.lang (Plus r1 r2) = eval (Union f g) v" by simp
   then show ?case by blast
 next
   case (4 f g)
@@ -271,61 +269,66 @@ next
 qed simp_all
 
 
-(* A regular function stays regular if all variables are substituted by regular functions *)
-lemma subst_reg_fun:
-  assumes "regular_fun f"
-      and "\<forall>x \<in> vars f. regular_fun (upd x)"
-    shows "regular_fun (subst upd f)"
-  using assms by (induction f rule: regular_fun.induct) simp_all
+text \<open>A \<open>reg_eval\<close> regular language expression stays \<open>reg_eval\<close> if all variables are substituted
+by \<open>reg_eval\<close> regular language expressions\<close>
+lemma subst_reg_eval:
+  assumes "reg_eval f"
+      and "\<forall>x \<in> vars f. reg_eval (upd x)"
+    shows "reg_eval (subst upd f)"
+  using assms by (induction f rule: reg_eval.induct) simp_all
 
 
-lemma subst_reg_fun_update:
-  assumes "regular_fun f"
-      and "regular_fun g"
-    shows "regular_fun (subst (Var(x := g)) f)"
-  using assms subst_reg_fun fun_upd_def by (metis regular_fun.simps(1))
+lemma subst_reg_eval_update:
+  assumes "reg_eval f"
+      and "reg_eval g"
+    shows "reg_eval (subst (Var(x := g)) f)"
+  using assms subst_reg_eval fun_upd_def by (metis reg_eval.simps(1))
 
+
+text \<open>For any finite union of \<open>reg_eval\<close> regular language expressions exists a \<open>reg_eval\<close> regular
+language expression\<close>
 
 lemma finite_Union_regular_aux:
-  "\<forall>f \<in> set fs. regular_fun f \<Longrightarrow> \<exists>g. regular_fun g \<and> \<Union>(vars ` set fs) = vars g
+  "\<forall>f \<in> set fs. reg_eval f \<Longrightarrow> \<exists>g. reg_eval g \<and> \<Union>(vars ` set fs) = vars g
                                       \<and> (\<forall>v. (\<Union>f \<in> set fs. eval f v) = eval g v)"
 proof (induction fs)
   case Nil
   then show ?case using emptyset_regular by fastforce
 next
   case (Cons f1 fs)
-  then obtain g where *: "regular_fun g \<and> \<Union>(vars ` set fs) = vars g
+  then obtain g where *: "reg_eval g \<and> \<Union>(vars ` set fs) = vars g
                           \<and> (\<forall>v. (\<Union>f\<in>set fs. eval f v) = eval g v)" by auto
-  let ?g' = "Union2 f1 g"
-  from Cons.prems * have "regular_fun ?g' \<and> \<Union> (vars ` set (f1 # fs)) = vars ?g'
+  let ?g' = "Union f1 g"
+  from Cons.prems * have "reg_eval ?g' \<and> \<Union> (vars ` set (f1 # fs)) = vars ?g'
       \<and> (\<forall>v. (\<Union>f\<in>set (f1 # fs). eval f v) = eval ?g' v)" by simp
   then show ?case by blast
 qed
 
-
 lemma finite_Union_regular:
   assumes "finite F"
-      and "\<forall>f \<in> F. regular_fun f"
-    shows "\<exists>g. regular_fun g \<and> \<Union>(vars ` F) = vars g \<and> (\<forall>v. (\<Union>f\<in>F. eval f v) = eval g v)"
+      and "\<forall>f \<in> F. reg_eval f"
+    shows "\<exists>g. reg_eval g \<and> \<Union>(vars ` F) = vars g \<and> (\<forall>v. (\<Union>f\<in>F. eval f v) = eval g v)"
   using assms finite_Union_regular_aux finite_list by metis
 
 
 
-section \<open>Constant functions\<close>
+section \<open>Constant regular language functions\<close>
 
-abbreviation const_fun :: "'a lfun \<Rightarrow> bool" where
-  "const_fun f \<equiv> vars f = {}"
+text \<open>A regular language expression is constant iff it contains no variables\<close>
+abbreviation const_rlexp :: "'a rlexp \<Rightarrow> bool" where
+  "const_rlexp f \<equiv> vars f = {}"
 
-lemma const_fun_lang: "const_fun f \<Longrightarrow> \<exists>l. \<forall>v. eval f v = l"
-proof (induction f)
-  case (UnionC x)
-  then show ?case by (metis emptyE eval_vars)
-qed auto
+text \<open>A constant regular language expression always evaluates to the same language, independent on
+the valuation\<close>
+lemma const_rlexp_lang: "const_rlexp f \<Longrightarrow> \<exists>l. \<forall>v. eval f v = l"
+  by (induction f) auto
 
-lemma const_fun_regular_lang:
-  assumes "const_fun f"
-      and "regular_fun f"
+text \<open>A regular language expression which is constant and \<open>reg_eval\<close>, evaluates to some regular
+language, independent on the valuation\<close>
+lemma const_rlexp_regular_lang:
+  assumes "const_rlexp f"
+      and "reg_eval f"
     shows "\<exists>l. regular_lang l \<and> (\<forall>v. eval f v = l)"
-  using assms const_fun_lang regular_fun_regular by fastforce
+  using assms const_rlexp_lang reg_eval_regular by fastforce
 
 end
