Parikh/Pilling.thy
@@ -2,112 +2,124 @@ theory Pilling
   imports 
     "../CFG"
     "../CFL"
-    "./Lfun"
-    "./Parikh_Img"
-    "./Eq_Sys"
+    "Lfun"
+    "Parikh_Img"
+    "Eq_Sys"
     "Regular-Sets.Regular_Set"
     "Regular-Sets.Regular_Exp"
 begin
 
 
-section \<open>Special representation of regular functions\<close>
-
-(* We first show that for every regular function f there is a representation of the form
-   (3) (see Pilling's paper, we call it regular_fun' in the following)
-   that has the same parikh image as f
-*)
-
-definition regular_fun' :: "nat \<Rightarrow> 'a lfun \<Rightarrow> bool" where
-  "regular_fun' x f \<equiv> \<exists>p q. regular_fun p \<and> regular_fun q \<and>
-    f = Union2 p (Concat q (Var x)) \<and> x \<notin> vars p"
-
-lemma "regular_fun' x f \<Longrightarrow> regular_fun f"
-  unfolding regular_fun'_def by fastforce
+text \<open>We prove Parikh's theorem, closely following Pilling's proof (TODO: citation). The rough
+idea is as follows: Each CFG can be interpreted as a system of equations. Pilling shows that
+there is a regular solution to this system if one applies the Parikh image on both sides of each
+equation (in the following, we will call this modified system of equations the "commutative system
+of equations") and that this solution is furthermore minimal. Since the CFL minimally solves
+the commutative system of equations as well (see Eq_Sys.thy for a proof), the Parikh image of the
+CFL and the regular solution must be identical, proving Parikh's theorem.\<close>
 
 
-text \<open>Every regular function can be represented as regular_fun':\<close>
+section \<open>Special representation of regular language expressions\<close>
 
-lemma regular_fun_regular_fun'_Variable: "\<exists>f'. regular_fun' x f' \<and> vars f' = vars (Var y) \<union> {x}
+text \<open>To each regular language expression and variable \<open>x\<close> corresponds a second regular language
+expression with the same Parikh image and of the form \<open>p \<union> q @@ Var x\<close> (see equation 3 in Pilling's paper)
+where p does not depend on x. We call regular language expressions of this form "bipartite regular
+language expressions":\<close>
+definition bipart_rlexp :: "nat \<Rightarrow> 'a rlexp \<Rightarrow> bool" where
+  "bipart_rlexp x f \<equiv> \<exists>p q. reg_eval p \<and> reg_eval q \<and>
+    f = Union p (Concat q (Var x)) \<and> x \<notin> vars p"
+
+
+text \<open>All bipartite regular language expressions evaluate to regular languages:\<close>
+lemma "bipart_rlexp x f \<Longrightarrow> reg_eval f"
+  unfolding bipart_rlexp_def by fastforce
+
+
+text \<open>For each reg_eval regular language expression and variable \<open>x\<close>, there exists a bipartite
+regular language expression with identical Parikh image and almost identical set of variables.
+We first prove some auxiliary lemmas\<close>
+
+lemma reg_eval_bipart_rlexp_Variable: "\<exists>f'. bipart_rlexp x f' \<and> vars f' = vars (Var y) \<union> {x}
                                         \<and> (\<forall>v. parikh_img (eval (Var y) v) = parikh_img (eval f' v))"
 proof (cases "x = y")
-let ?f' = "Union2 (Const {}) (Concat (Const {[]}) (Var x))"
+let ?f' = "Union (Const {}) (Concat (Const {[]}) (Var x))"
   case True
-  then have "regular_fun' x ?f'"
-    unfolding regular_fun'_def using emptyset_regular epsilon_regular by fastforce
+  then have "bipart_rlexp x ?f'"
+    unfolding bipart_rlexp_def using emptyset_regular epsilon_regular by fastforce
   moreover have "eval ?f' v = eval (Var y) v" for v :: "'a valuation" using True by simp
   moreover have "vars ?f' = vars (Var y) \<union> {x}" using True by simp
   ultimately show ?thesis by metis
 next
-  let ?f' = "Union2 (Var y) (Concat (Const {}) (Var x))"
+  let ?f' = "Union (Var y) (Concat (Const {}) (Var x))"
   case False
-  then have "regular_fun' x ?f'"
-    unfolding regular_fun'_def using emptyset_regular epsilon_regular by fastforce
+  then have "bipart_rlexp x ?f'"
+    unfolding bipart_rlexp_def using emptyset_regular epsilon_regular by fastforce
   moreover have "eval ?f' v = eval (Var y) v" for v :: "'a valuation" using False by simp
   moreover have "vars ?f' = vars (Var y) \<union> {x}" by simp
   ultimately show ?thesis by metis
 qed
 
-lemma regular_fun_regular_fun'_Const:
+lemma reg_eval_bipart_rlexp_Const:
   assumes "regular_lang l"
-    shows "\<exists>f'. regular_fun' x f' \<and> vars f' = vars (Const l) \<union> {x}
+    shows "\<exists>f'. bipart_rlexp x f' \<and> vars f' = vars (Const l) \<union> {x}
                 \<and> (\<forall>v. parikh_img (eval (Const l) v) = parikh_img (eval f' v))"
 proof -
-  let ?f' = "Union2 (Const l) (Concat (Const {}) (Var x))"
-  have "regular_fun' x ?f'"
-    unfolding regular_fun'_def using assms emptyset_regular by simp
+  let ?f' = "Union (Const l) (Concat (Const {}) (Var x))"
+  have "bipart_rlexp x ?f'"
+    unfolding bipart_rlexp_def using assms emptyset_regular by simp
   moreover have "eval ?f' v = eval (Const l) v" for v :: "'a valuation" by simp
   moreover have "vars ?f' = vars (Const l) \<union> {x}" by simp 
   ultimately show ?thesis by metis
 qed
 
-lemma regular_fun_regular_fun'_Union2:
-  assumes "\<exists>f'. regular_fun' x f' \<and> vars f' = vars f1 \<union> {x} \<and>
+lemma reg_eval_bipart_rlexp_Union:
+  assumes "\<exists>f'. bipart_rlexp x f' \<and> vars f' = vars f1 \<union> {x} \<and>
                 (\<forall>v. parikh_img (eval f1 v) = parikh_img (eval f' v))"
-          "\<exists>f'. regular_fun' x f' \<and> vars f' = vars f2 \<union> {x} \<and>
+          "\<exists>f'. bipart_rlexp x f' \<and> vars f' = vars f2 \<union> {x} \<and>
                 (\<forall>v. parikh_img (eval f2 v) = parikh_img (eval f' v))"
-    shows "\<exists>f'. regular_fun' x f' \<and> vars f' = vars (Union2 f1 f2) \<union> {x} \<and>
-                (\<forall>v. parikh_img (eval (Union2 f1 f2) v) = parikh_img (eval f' v))"
+    shows "\<exists>f'. bipart_rlexp x f' \<and> vars f' = vars (Union f1 f2) \<union> {x} \<and>
+                (\<forall>v. parikh_img (eval (Union f1 f2) v) = parikh_img (eval f' v))"
 proof -
-  from assms obtain f1' f2' where f1'_intro: "regular_fun' x f1' \<and> vars f1' = vars f1 \<union> {x} \<and>
+  from assms obtain f1' f2' where f1'_intro: "bipart_rlexp x f1' \<and> vars f1' = vars f1 \<union> {x} \<and>
       (\<forall>v. parikh_img (eval f1 v) = parikh_img (eval f1' v))"
-    and f2'_intro: "regular_fun' x f2' \<and> vars f2' = vars f2 \<union> {x} \<and>
+    and f2'_intro: "bipart_rlexp x f2' \<and> vars f2' = vars f2 \<union> {x} \<and>
       (\<forall>v. parikh_img (eval f2 v) = parikh_img (eval f2' v))"
     by auto
-  then obtain p1 q1 p2 q2 where p1_q1_intro: "regular_fun p1 \<and> regular_fun q1 \<and>
-    f1' = Union2 p1 (Concat q1 (Var x)) \<and> (\<forall>y \<in> vars p1. y \<noteq> x)"
-    and p2_q2_intro: "regular_fun p2 \<and> regular_fun q2 \<and> f2' = Union2 p2 (Concat q2 (Var x)) \<and>
-    (\<forall>y \<in> vars p2. y \<noteq> x)" unfolding regular_fun'_def by auto
+  then obtain p1 q1 p2 q2 where p1_q1_intro: "reg_eval p1 \<and> reg_eval q1 \<and>
+    f1' = Union p1 (Concat q1 (Var x)) \<and> (\<forall>y \<in> vars p1. y \<noteq> x)"
+    and p2_q2_intro: "reg_eval p2 \<and> reg_eval q2 \<and> f2' = Union p2 (Concat q2 (Var x)) \<and>
+    (\<forall>y \<in> vars p2. y \<noteq> x)" unfolding bipart_rlexp_def by auto
 
-  let ?f' = "Union2 (Union2 p1 p2) (Concat (Union2 q1 q2) (Var x))"
-  have "regular_fun' x ?f'" unfolding regular_fun'_def using p1_q1_intro p2_q2_intro by auto
-  moreover have "parikh_img (eval ?f' v) = parikh_img (eval (Union2 f1 f2) v)" for v
+  let ?f' = "Union (Union p1 p2) (Concat (Union q1 q2) (Var x))"
+  have "bipart_rlexp x ?f'" unfolding bipart_rlexp_def using p1_q1_intro p2_q2_intro by auto
+  moreover have "parikh_img (eval ?f' v) = parikh_img (eval (Union f1 f2) v)" for v
     using p1_q1_intro p2_q2_intro f1'_intro f2'_intro
     by (simp add: conc_Un_distrib(2) sup_assoc sup_left_commute)
   moreover from f1'_intro f2'_intro p1_q1_intro p2_q2_intro
-    have "vars ?f' = vars (Union2 f1 f2) \<union> {x}" by auto
+    have "vars ?f' = vars (Union f1 f2) \<union> {x}" by auto
   ultimately show ?thesis by metis
 qed
 
-lemma regular_fun_regular_fun'_Concat:
-  assumes "\<exists>f'. regular_fun' x f' \<and> vars f' = vars f1 \<union> {x} \<and>
+lemma reg_eval_bipart_rlexp_Concat:
+  assumes "\<exists>f'. bipart_rlexp x f' \<and> vars f' = vars f1 \<union> {x} \<and>
                 (\<forall>v. parikh_img (eval f1 v) = parikh_img (eval f' v))"
-          "\<exists>f'. regular_fun' x f' \<and> vars f' = vars f2 \<union> {x} \<and>
+          "\<exists>f'. bipart_rlexp x f' \<and> vars f' = vars f2 \<union> {x} \<and>
                 (\<forall>v. parikh_img (eval f2 v) = parikh_img (eval f' v))"
-    shows "\<exists>f'. regular_fun' x f' \<and> vars f' = vars (Concat f1 f2) \<union> {x} \<and>
+    shows "\<exists>f'. bipart_rlexp x f' \<and> vars f' = vars (Concat f1 f2) \<union> {x} \<and>
                 (\<forall>v. parikh_img (eval (Concat f1 f2) v) = parikh_img (eval f' v))"
 proof -
-  from assms obtain f1' f2' where f1'_intro: "regular_fun' x f1' \<and> vars f1' = vars f1 \<union> {x} \<and>
+  from assms obtain f1' f2' where f1'_intro: "bipart_rlexp x f1' \<and> vars f1' = vars f1 \<union> {x} \<and>
       (\<forall>v. parikh_img (eval f1 v) = parikh_img (eval f1' v))"
-    and f2'_intro: "regular_fun' x f2' \<and> vars f2' = vars f2 \<union> {x} \<and>
+    and f2'_intro: "bipart_rlexp x f2' \<and> vars f2' = vars f2 \<union> {x} \<and>
       (\<forall>v. parikh_img (eval f2 v) = parikh_img (eval f2' v))"
     by auto
-  then obtain p1 q1 p2 q2 where p1_q1_intro: "regular_fun p1 \<and> regular_fun q1 \<and>
-    f1' = Union2 p1 (Concat q1 (Var x)) \<and> (\<forall>y \<in> vars p1. y \<noteq> x)"
-    and p2_q2_intro: "regular_fun p2 \<and> regular_fun q2 \<and> f2' = Union2 p2 (Concat q2 (Var x)) \<and>
-    (\<forall>y \<in> vars p2. y \<noteq> x)" unfolding regular_fun'_def by auto
+  then obtain p1 q1 p2 q2 where p1_q1_intro: "reg_eval p1 \<and> reg_eval q1 \<and>
+    f1' = Union p1 (Concat q1 (Var x)) \<and> (\<forall>y \<in> vars p1. y \<noteq> x)"
+    and p2_q2_intro: "reg_eval p2 \<and> reg_eval q2 \<and> f2' = Union p2 (Concat q2 (Var x)) \<and>
+    (\<forall>y \<in> vars p2. y \<noteq> x)" unfolding bipart_rlexp_def by auto
 
-  let ?q' = "Union2 (Concat q1 (Concat (Var x) q2)) (Union2 (Concat p1 q2) (Concat q1 p2))"
-  let ?f' = "Union2 (Concat p1 p2) (Concat ?q' (Var x))"
+  let ?q' = "Union (Concat q1 (Concat (Var x) q2)) (Union (Concat p1 q2) (Concat q1 p2))"
+  let ?f' = "Union (Concat p1 p2) (Concat ?q' (Var x))"
 
   have "\<forall>v. (parikh_img (eval (Concat f1 f2) v) = parikh_img (eval ?f' v))"
   proof (rule allI)
@@ -117,7 +129,7 @@ proof -
 
     have "parikh_img (eval (Concat f1 f2) v) = parikh_img ((eval p1 v \<union> eval q1 v @@ v x) @@ eval f2 v)"
       using p1_q1_intro f1'_intro
-      by (metis eval.simps(1) eval.simps(3) eval.simps(5) parikh_conc_right)
+      by (metis eval.simps(1) eval.simps(3) eval.simps(4) parikh_conc_right)
     also have "\<dots> = parikh_img (eval p1 v @@ eval f2 v \<union> eval q1 v @@ v x @@ eval f2 v)"
       by (simp add: conc_Un_distrib(2) conc_assoc)
     also have "\<dots> = parikh_img (eval p1 v @@ (eval p2 v \<union> eval q2 v @@ v x)
@@ -133,32 +145,32 @@ proof -
       by (simp add: Un_commute)
     finally show "parikh_img (eval (Concat f1 f2) v) = parikh_img (eval ?f' v)" .
   qed
-  moreover have "regular_fun' x ?f'" unfolding regular_fun'_def using p1_q1_intro p2_q2_intro by auto
+  moreover have "bipart_rlexp x ?f'" unfolding bipart_rlexp_def using p1_q1_intro p2_q2_intro by auto
   moreover from f1'_intro f2'_intro p1_q1_intro p2_q2_intro
     have "vars ?f' = vars (Concat f1 f2) \<union> {x}" by auto
   ultimately show ?thesis by metis
 qed
 
-lemma regular_fun_regular_fun'_Star:
-  assumes "\<exists>f'. regular_fun' x f' \<and> vars f' = vars f \<union> {x}
+lemma reg_eval_bipart_rlexp_Star:
+  assumes "\<exists>f'. bipart_rlexp x f' \<and> vars f' = vars f \<union> {x}
                 \<and> (\<forall>v. parikh_img (eval f v) = parikh_img (eval f' v))"
-  shows "\<exists>f'. regular_fun' x f' \<and> vars f' = vars (Star f) \<union> {x}
+  shows "\<exists>f'. bipart_rlexp x f' \<and> vars f' = vars (Star f) \<union> {x}
                 \<and> (\<forall>v. parikh_img (eval (Star f) v) = parikh_img (eval f' v))"
 proof -
-  from assms obtain f' where f'_intro: "regular_fun' x f' \<and> vars f' = vars f \<union> {x} \<and>
+  from assms obtain f' where f'_intro: "bipart_rlexp x f' \<and> vars f' = vars f \<union> {x} \<and>
       (\<forall>v. parikh_img (eval f v) = parikh_img (eval f' v))" by auto
-  then obtain p q where p_q_intro: "regular_fun p \<and> regular_fun q \<and>
-    f' = Union2 p (Concat q (Var x)) \<and> (\<forall>y \<in> vars p. y \<noteq> x)" unfolding regular_fun'_def by auto
+  then obtain p q where p_q_intro: "reg_eval p \<and> reg_eval q \<and>
+    f' = Union p (Concat q (Var x)) \<and> (\<forall>y \<in> vars p. y \<noteq> x)" unfolding bipart_rlexp_def by auto
 
   let ?q_new = "Concat (Star p) (Concat (Star (Concat q (Var x))) (Concat (Star (Concat q (Var x))) q))"
-  let ?f_new = "Union2 (Star p) (Concat ?q_new (Var x))"
+  let ?f_new = "Union (Star p) (Concat ?q_new (Var x))"
 
   have "\<forall>v. (parikh_img (eval (Star f) v) = parikh_img (eval ?f_new v))"
   proof (rule allI)
     fix v
     have "parikh_img (eval (Star f) v) = parikh_img (star (eval p v \<union> eval q v @@ v x))"
       using f'_intro parikh_star_mono_eq p_q_intro
-      by (metis eval.simps(1) eval.simps(3) eval.simps(5) eval.simps(6))
+      by (metis eval.simps(1) eval.simps(3) eval.simps(4) eval.simps(5))
     also have "\<dots> = parikh_img (star (eval p v) @@ star (eval q v @@ v x))"
       using parikh_img_star by blast
     also have "\<dots> = parikh_img (star (eval p v) @@
@@ -174,73 +186,80 @@ proof -
     also have "\<dots> = parikh_img (eval ?f_new v)" by (simp add: conc_assoc)
     finally show "parikh_img (eval (Star f) v) = parikh_img (eval ?f_new v)" .
   qed
-  moreover have "regular_fun' x ?f_new" unfolding regular_fun'_def using p_q_intro by fastforce
+  moreover have "bipart_rlexp x ?f_new" unfolding bipart_rlexp_def using p_q_intro by fastforce
   moreover from f'_intro p_q_intro have "vars ?f_new = vars (Star f) \<union> {x}" by auto
   ultimately show ?thesis by metis
 qed
 
-(* Every regular function can be represented in form (3),
-   as long as we only care for the Parikh image
-*)
-lemma regular_fun_regular_fun': "regular_fun f \<Longrightarrow>
-    \<exists>f'. regular_fun' x f' \<and> vars f' = vars f \<union> {x} \<and>
+text \<open>The actual lemma:\<close>
+lemma reg_eval_bipart_rlexp: "reg_eval f \<Longrightarrow>
+    \<exists>f'. bipart_rlexp x f' \<and> vars f' = vars f \<union> {x} \<and>
          (\<forall>s. parikh_img (eval f s) = parikh_img (eval f' s))"
-proof (induction f rule: regular_fun.induct)
+proof (induction f rule: reg_eval.induct)
   case (1 uu)
-  from regular_fun_regular_fun'_Variable show ?case by blast
+  from reg_eval_bipart_rlexp_Variable show ?case by blast
 next
   case (2 l)
   then have "regular_lang l" by simp
-  from regular_fun_regular_fun'_Const[OF this] show ?case by blast
+  from reg_eval_bipart_rlexp_Const[OF this] show ?case by blast
 next
   case (3 f g)
-  then have "\<exists>f'. regular_fun' x f' \<and> vars f' = vars f \<union> {x} \<and> (\<forall>v. parikh_img (eval f v) = parikh_img (eval f' v))"
-            "\<exists>f'. regular_fun' x f' \<and> vars f' = vars g \<union> {x} \<and> (\<forall>v. parikh_img (eval g v) = parikh_img (eval f' v))"
+  then have "\<exists>f'. bipart_rlexp x f' \<and> vars f' = vars f \<union> {x} \<and> (\<forall>v. parikh_img (eval f v) = parikh_img (eval f' v))"
+            "\<exists>f'. bipart_rlexp x f' \<and> vars f' = vars g \<union> {x} \<and> (\<forall>v. parikh_img (eval g v) = parikh_img (eval f' v))"
     by auto
-  from regular_fun_regular_fun'_Union2[OF this] show ?case by blast
+  from reg_eval_bipart_rlexp_Union[OF this] show ?case by blast
 next
   case (4 f g)
-  then have "\<exists>f'. regular_fun' x f' \<and> vars f' = vars f \<union> {x} \<and> (\<forall>v. parikh_img (eval f v) = parikh_img (eval f' v))"
-            "\<exists>f'. regular_fun' x f' \<and> vars f' = vars g \<union> {x} \<and> (\<forall>v. parikh_img (eval g v) = parikh_img (eval f' v))"
+  then have "\<exists>f'. bipart_rlexp x f' \<and> vars f' = vars f \<union> {x} \<and> (\<forall>v. parikh_img (eval f v) = parikh_img (eval f' v))"
+            "\<exists>f'. bipart_rlexp x f' \<and> vars f' = vars g \<union> {x} \<and> (\<forall>v. parikh_img (eval g v) = parikh_img (eval f' v))"
     by auto
-  from regular_fun_regular_fun'_Concat[OF this] show ?case by blast
+  from reg_eval_bipart_rlexp_Concat[OF this] show ?case by blast
 next
   case (5 f)
-  then have "\<exists>f'. regular_fun' x f' \<and> vars f' = vars f \<union> {x} \<and> (\<forall>v. parikh_img (eval f v) = parikh_img (eval f' v))"
+  then have "\<exists>f'. bipart_rlexp x f' \<and> vars f' = vars f \<union> {x} \<and> (\<forall>v. parikh_img (eval f v) = parikh_img (eval f' v))"
     by auto
-  from regular_fun_regular_fun'_Star[OF this] show ?case by blast
-qed simp
+  from reg_eval_bipart_rlexp_Star[OF this] show ?case by blast
+qed
 
 
 section \<open>Minimal solution\<close>
+
+text \<open>We show that any commutative system of equations has some minimal solution which is reg_eval\<close>
+
 
 subsection \<open>Minimal solution for a single equation\<close>
 
 (* We show that F(E)*E (in the following q(p)*p is a minimal solution) *)
 
-locale of_form_regular_fun' =
+text \<open>We first prove that every bipartite regular language expression for the variable \<open>x\<close> has
+some minimal solution which is reg_eval\<close>
+
+locale single_bipartite_eq =
   fixes x :: "nat"
-  fixes p :: "'a lfun"
-  fixes q :: "'a lfun"
-  assumes p_reg:      "regular_fun p"
-  assumes q_reg:      "regular_fun q"
+  fixes p :: "'a rlexp"
+  fixes q :: "'a rlexp"
+  assumes p_reg:      "reg_eval p"
+  assumes q_reg:      "reg_eval q"
   assumes x_not_in_p: "x \<notin> vars p"
 begin
 
-abbreviation "eq \<equiv> Union2 p (Concat q (Var x))"
+text \<open>The equation\<close>
+abbreviation "eq \<equiv> Union p (Concat q (Var x))"
+
+text \<open>The solution\<close>
 abbreviation "sol \<equiv> Concat (Star (subst (Var(x := p)) q)) p"
 
 
-(* F(E)*E is a regular function *)
-lemma sol_is_reg: "regular_fun sol"
+text \<open>\<open>sol\<close> is a reg_eval regular language expression\<close>
+lemma sol_is_reg: "reg_eval sol"
 proof -
-  from p_reg q_reg have r_reg: "regular_fun (subst (Var(x := p)) q)"
-    using subst_reg_fun_update by auto
-  with p_reg show "regular_fun sol" by auto
+  from p_reg q_reg have r_reg: "reg_eval (subst (Var(x := p)) q)"
+    using subst_reg_eval_update by auto
+  with p_reg show "reg_eval sol" by auto
 qed
 
 
-(* F(E)*E contains only variables which also appear in the equation, except x *)
+text \<open>\<open>sol\<close> contains only variables which also appear in the equation and it does not contain \<open>x\<close>\<close>
 lemma sol_vars: "vars sol \<subseteq> vars eq - {x}"
 proof -
   let ?upd = "Var(x := p)"
@@ -266,7 +285,7 @@ proof -
 qed
 
 
-(* F(E)*E is a solution of equation (3) from the paper (with \<supseteq> instead of =) *)
+text \<open>\<open>sol\<close> is a partial solution of the equation\<close>
 lemma sol_is_sol_ineq: "partial_sol_ineq x eq sol"
 unfolding partial_sol_ineq_def proof (rule allI, rule impI)
   fix v
@@ -277,9 +296,8 @@ unfolding partial_sol_ineq_def proof (rule allI, rule impI)
   let ?q_subst = "subst ?upd q"
   let ?eq_subst = "subst ?upd eq"
 
-  from sol_is_reg have r_reg: "regular_fun ?r" unfolding fun_upd_def by fastforce
   have homogeneous_app: "parikh_img (eval ?q_subst v) \<subseteq> parikh_img (eval (Concat (Star ?r) ?r) v)"
-    using reg_fun_homogeneous[OF q_reg r_reg p_reg] by blast
+    using rlexp_homogeneous by blast
 
   from x_not_in_p have "eval (subst ?upd p) v = eval p v" using eval_vars_subst[of p] by simp
   then have "parikh_img (eval ?eq_subst v) = parikh_img (eval p v \<union> eval ?q_subst v @@ eval sol v)"
@@ -304,6 +322,7 @@ unfolding partial_sol_ineq_def proof (rule allI, rule impI)
 qed
 
 
+text \<open>The equation does not have any partial solution smaller than \<open>sol\<close>\<close>
 lemma sol_is_minimal:
   assumes is_sol:    "solves_ineq_comm x eq v"
       and sol'_s:    "v x = eval sol' v"
@@ -320,40 +339,14 @@ proof -
   then have "parikh_img (eval (Star (subst (Var(x := p)) q)) v) \<subseteq> parikh_img (eval (Star q) v)"
     using parikh_star_mono by auto
   then have "parikh_img (eval sol v) \<subseteq> parikh_img (eval (Concat (Star q) p) v)"
-    using parikh_conc_right_subset by (metis eval.simps(5))
+    using parikh_conc_right_subset by (metis eval.simps(4))
 
   with 1 show ?thesis by fast
 qed
 
-
-(* TODO: should not be needed, right? *)
-(* F(E)*E solves equation (3) from the paper (this time with =) *)
-(*lemma sol_is_sol_eq: "partial_sol_eq x eq sol"
-unfolding partial_sol_eq_def proof
-  fix s
-
-  let ?r = "subst q (\<lambda>y. if y = x then p else V y)"
-  let ?upd = "\<lambda>y. if y = x then sol else V y"
-  let ?upd_subst = "\<lambda>y. if y = x then subst eq ?upd else V y"
-
-  have "parikh_img (eval (subst eq ?upd_subst) s) \<subseteq> parikh_img (eval (subst eq ?upd) s)" for s
-  proof -
-    fix s
-    from sol_is_sol_ineq have "parikh_img (eval (subst eq ?upd) s) \<subseteq> parikh_img (eval sol s)"
-      unfolding partial_sol_ineq_def sorry (* by blast *)
-    then show "parikh_img (eval (subst eq ?upd_subst) s) \<subseteq> parikh_img (eval (subst eq ?upd) s)"
-      using parikh_img_subst_mono[of ?upd_subst s ?upd eq] by auto
-  qed
-  then have "partial_sol_ineq x eq (subst eq ?upd)" unfolding partial_sol_ineq_def by auto
-  then have "parikh_img (eval sol s) \<subseteq> parikh_img (eval (subst eq ?upd) s)"
-    using sol_is_minimal by blast
-  with sol_is_sol_ineq show "parikh_img (eval (subst eq ?upd) s) = parikh_img (eval sol s)"
-    unfolding partial_sol_ineq_def by blast
-qed*)
-
-
+text \<open>In summary, \<open>sol\<close> is a minimal partial solution and it is reg_eval\<close>
 lemma sol_is_minimal_reg_sol:
-  "regular_fun sol \<and> partial_min_sol_one_ineq x eq sol"
+  "reg_eval sol \<and> partial_min_sol_one_ineq x eq sol"
   unfolding partial_min_sol_one_ineq_def
   using sol_is_reg sol_vars sol_is_sol_ineq sol_is_minimal
   by blast
@@ -361,45 +354,57 @@ lemma sol_is_minimal_reg_sol:
 end
 
 
-(* Given equation (2), there exists a regular minimal solution *)
+text \<open>Every equation (not necessarily bipartite) has some minimal partial solution which is reg_eval\<close>
 lemma exists_minimal_reg_sol:
-  assumes eq_reg: "regular_fun eq"
-  shows "\<exists>sol. regular_fun sol \<and> partial_min_sol_one_ineq x eq sol"
+  assumes eq_reg: "reg_eval eq"
+  shows "\<exists>sol. reg_eval sol \<and> partial_min_sol_one_ineq x eq sol"
 proof -
-  from regular_fun_regular_fun'[OF eq_reg] obtain eq'
-    where eq'_intro: "regular_fun' x eq' \<and> vars eq' = vars eq \<union> {x} \<and>
+  from reg_eval_bipart_rlexp[OF eq_reg] obtain eq'
+    where eq'_intro: "bipart_rlexp x eq' \<and> vars eq' = vars eq \<union> {x} \<and>
                     (\<forall>v. parikh_img (eval eq v) = parikh_img (eval eq' v))" by blast
   then obtain p q
-    where p_q_intro: "regular_fun p \<and> regular_fun q \<and> eq' = Union2 p (Concat q (Var x)) \<and> x \<notin> vars p"
-    unfolding regular_fun'_def by blast
+    where p_q_intro: "reg_eval p \<and> reg_eval q \<and> eq' = Union p (Concat q (Var x)) \<and> x \<notin> vars p"
+    unfolding bipart_rlexp_def by blast
 
   let ?sol = "Concat (Star (subst (Var(x := p)) q)) p"
-  from p_q_intro have sol_prop: "regular_fun ?sol \<and> partial_min_sol_one_ineq x eq' ?sol"
-    using of_form_regular_fun'.sol_is_minimal_reg_sol unfolding of_form_regular_fun'_def by blast
+  from p_q_intro have sol_prop: "reg_eval ?sol \<and> partial_min_sol_one_ineq x eq' ?sol"
+    using single_bipartite_eq.sol_is_minimal_reg_sol unfolding single_bipartite_eq_def by blast
   with eq'_intro have "partial_min_sol_one_ineq x eq ?sol"
     using same_min_sol_if_same_parikh_img by blast
   with sol_prop show ?thesis by blast
 qed
 
 
-subsection \<open>Minimal solution of the whole equation system\<close>
+subsection \<open>Minimal solution of the whole system of equations\<close>
 
-locale minimal_sol_one_eq =
+text \<open>Now, we will prove that the whole commutative system of equations has some minimal solution
+which is regular. For this purpose, we will show by induction that the first \<open>r\<close> equations have
+some minimal partial solution which is reg_eval.
+First, we show the centerpiece of the induction step: If a reg_eval and minimal partial solution
+\<open>sols\<close> exists for the first \<open>r\<close> equations and furthermore a reg_eval and minimal partial solution
+\<open>sol_r\<close> exists for the \<open>r\<close>-th equation, then there exists a reg_eval and minimal partial solution
+for the first \<open>Suc r\<close> equations as well.\<close>
+
+locale min_sol_induction_step =
   fixes r :: nat
     and sys :: "'a eq_sys"
-    and sols :: "nat \<Rightarrow> 'a lfun"
-    and sol_r :: "'a lfun"
-  assumes eqs_reg:      "\<forall>eq \<in> set sys. regular_fun eq"
+    and sols :: "nat \<Rightarrow> 'a rlexp"
+    and sol_r :: "'a rlexp"
+  assumes eqs_reg:      "\<forall>eq \<in> set sys. reg_eval eq"
       and sys_valid:    "\<forall>eq \<in> set sys. \<forall>x \<in> vars eq. x < length sys"
       and r_valid:      "r < length sys"
       and sols_is_sol:  "partial_min_sol_ineq_sys r sys sols"
-      and sols_reg:     "\<forall>i. regular_fun (sols i)"
+      and sols_reg:     "\<forall>i. reg_eval (sols i)"
       and sol_r_is_sol: "partial_min_sol_one_ineq r (subst_sys sols sys ! r) sol_r"
-      and sol_r_reg:    "regular_fun sol_r"
+      and sol_r_reg:    "reg_eval sol_r"
 begin
 
 
+text \<open>Substitute the partial solutions for the first \<open>r\<close> equations into the system of equations:\<close>
 abbreviation "sys' \<equiv> subst_sys sols sys"
+
+text \<open>The solution for the first \<open>Suc r\<close> equations. We retrieve it by substituting the partial
+solution of the \<open>r\<close>-th equation into the partial solutions for the first \<open>r\<close> equations:\<close>
 abbreviation "sols' \<equiv> \<lambda>i. subst (Var(r := sol_r)) (sols i)"
 
 
@@ -407,10 +412,12 @@ lemma sols'_r: "sols' r = sol_r"
   using sols_is_sol unfolding partial_min_sol_ineq_sys_def by simp
 
 
-lemma sols'_reg: "\<forall>i. regular_fun (sols' i)"
-  using sols_reg sol_r_reg using subst_reg_fun_update by blast
+text \<open>All regular language expressions in \<open>sols'\<close> are still reg_eval\<close>
+lemma sols'_reg: "\<forall>i. reg_eval (sols' i)"
+  using sols_reg sol_r_reg using subst_reg_eval_update by blast
 
 
+text \<open>\<open>sols'\<close> is a partial solution of the first \<open>Suc r\<close> equations\<close>
 lemma sols'_is_sol: "solution_ineq_sys (take (Suc r) sys) sols'"
 unfolding solution_ineq_sys_def proof (rule allI, rule impI)
   fix v
@@ -433,7 +440,7 @@ unfolding solution_ineq_sys_def proof (rule allI, rule impI)
     unfolding solves_ineq_sys_comm_def solves_ineq_comm_def by (auto simp add: less_Suc_eq)
 qed
 
-
+text \<open>There is no partial solution of the first \<open>Suc r\<close> equations which is smaller than \<open>sols'\<close>\<close>
 lemma sols'_min: "\<forall>sols2 v2. (\<forall>x. v2 x = eval (sols2 x) v2)
                    \<and> solves_ineq_sys_comm (take (Suc r) sys) v2
                    \<longrightarrow> (\<forall>i. parikh_img (eval (sols' i) v2) \<subseteq> parikh_img (v2 i))"
@@ -449,7 +456,7 @@ proof (rule allI | rule impI)+
     unfolding subst_sys_def using substitution_lemma[where f="sys ! r"]
     by (simp add: r_valid Suc_le_lessD)
   with sols_s2 have "parikh_img (eval (sys' ! r) v2) \<subseteq> parikh_img (eval (sys ! r) v2)"
-    using lfun_mono_parikh[of "sys ! r"] by auto
+    using rlexp_mono_parikh[of "sys ! r"] by auto
   with as have "solves_ineq_comm r (sys' ! r) v2"
     unfolding solves_ineq_sys_comm_def solves_ineq_comm_def using r_valid by force
   with as sol_r_is_sol have sol_r_min: "parikh_img (eval sol_r v2) \<subseteq> parikh_img (v2 r)"
@@ -458,7 +465,7 @@ proof (rule allI | rule impI)+
   let ?v' = "v2(r := eval sol_r v2)"
   from sol_r_min have "parikh_img (?v' i) \<subseteq> parikh_img (v2 i)" for i by simp
   with sols_s2 show "parikh_img (eval (sols' i) v2) \<subseteq> parikh_img (v2 i)"
-    using substitution_lemma_update[where f="sols i"] lfun_mono_parikh[of "sols i" ?v' v2] by force
+    using substitution_lemma_update[where f="sols i"] rlexp_mono_parikh[of "sols i" ?v' v2] by force
 qed
 
 
@@ -466,6 +473,8 @@ lemma sols'_vars_gt_r: "\<forall>i \<ge> Suc r. sols' i = Var i"
   using sols_is_sol unfolding partial_min_sol_ineq_sys_def by auto
 
 
+text \<open>No partial solution for one of the first \<open>Suc r\<close> equations depends on the variable \<open>r\<close> or 
+smaller variables or on variables which do not occur in the equation system\<close>
 lemma sols'_vars_leq_r: "\<forall>i < Suc r. \<forall>x \<in> vars (sols' i). x \<ge> Suc r \<and> x < length sys"
 proof -
   from sols_is_sol have "\<forall>i < r. \<forall>x \<in> vars (sols i). x \<ge> r \<and> x < length sys"
@@ -489,24 +498,29 @@ proof -
 qed
 
 
+text \<open>In summary, \<open>sols'\<close> is a minimal partial solution of the first \<open>Suc r\<close> equations\<close>
 lemma sols'_is_min_sol: "partial_min_sol_ineq_sys (Suc r) sys sols'"
   unfolding partial_min_sol_ineq_sys_def
   using sols'_is_sol sols'_min sols'_vars_gt_r sols'_vars_leq_r
   by blast
 
 
+text \<open>The centerpiece of the induction step: There exists a reg_eval and minimal partial solution
+for the first \<open>Suc r\<close> equations\<close>
 lemma exists_min_sol_Suc_r:
-  "\<exists>sols'. partial_min_sol_ineq_sys (Suc r) sys sols' \<and> (\<forall>i. regular_fun (sols' i))"
+  "\<exists>sols'. partial_min_sol_ineq_sys (Suc r) sys sols' \<and> (\<forall>i. reg_eval (sols' i))"
   using sols'_reg sols'_is_min_sol by blast
 
 end
 
 
+text \<open>The actual induction proof: For every \<open>r\<close>, there exists a reg_eval and minimal partial
+solution of the first \<open>r\<close> equations\<close>
 lemma exists_minimal_reg_sol_sys_aux:
-  assumes eqs_reg:   "\<forall>eq \<in> set sys. regular_fun eq"
+  assumes eqs_reg:   "\<forall>eq \<in> set sys. reg_eval eq"
       and sys_valid: "\<forall>eq \<in> set sys. \<forall>x \<in> vars eq. x < length sys"
       and r_valid:   "r \<le> length sys"   
-    shows            "\<exists>sols. partial_min_sol_ineq_sys r sys sols \<and> (\<forall>i. regular_fun (sols i))"
+    shows            "\<exists>sols. partial_min_sol_ineq_sys r sys sols \<and> (\<forall>i. reg_eval (sols i))"
 using assms proof (induction r)
   case 0
   have "solution_ineq_sys (take 0 sys) Var"
@@ -514,38 +528,40 @@ using assms proof (induction r)
   then show ?case unfolding partial_min_sol_ineq_sys_def by auto
 next
   case (Suc r)
-  then obtain sols where sols_intro: "partial_min_sol_ineq_sys r sys sols \<and> (\<forall>i. regular_fun (sols i))"
+  then obtain sols where sols_intro: "partial_min_sol_ineq_sys r sys sols \<and> (\<forall>i. reg_eval (sols i))"
     by auto
 
   let ?sys' = "subst_sys sols sys"
-  from eqs_reg Suc.prems have "regular_fun (sys ! r)" by simp
-  with sols_intro Suc.prems have sys_r_reg: "regular_fun (?sys' ! r)"
-    using subst_reg_fun[of "sys ! r"] subst_sys_subst[of r sys] by simp
+  from eqs_reg Suc.prems have "reg_eval (sys ! r)" by simp
+  with sols_intro Suc.prems have sys_r_reg: "reg_eval (?sys' ! r)"
+    using subst_reg_eval[of "sys ! r"] subst_sys_subst[of r sys] by simp
   then obtain sol_r where sol_r_intro:
-    "regular_fun sol_r \<and> partial_min_sol_one_ineq r (?sys' ! r) sol_r"
+    "reg_eval sol_r \<and> partial_min_sol_one_ineq r (?sys' ! r) sol_r"
     using exists_minimal_reg_sol by blast
 
-  with Suc sols_intro have "minimal_sol_one_eq r sys sols sol_r"
-    unfolding minimal_sol_one_eq_def by force
-  from minimal_sol_one_eq.exists_min_sol_Suc_r[OF this] show ?case by blast
+  with Suc sols_intro have "min_sol_induction_step r sys sols sol_r"
+    unfolding min_sol_induction_step_def by force
+  from min_sol_induction_step.exists_min_sol_Suc_r[OF this] show ?case by blast
 qed
 
 
+text \<open>As a consequence of the induction proof, there exists a regular and minimal (non-partial)
+solution for the whole system of equations\<close>
 lemma exists_minimal_reg_sol_sys:
-  assumes eqs_reg:   "\<forall>eq \<in> set sys. regular_fun eq"
+  assumes eqs_reg:   "\<forall>eq \<in> set sys. reg_eval eq"
       and sys_valid: "\<forall>eq \<in> set sys. \<forall>x \<in> vars eq. x < length sys"
     shows            "\<exists>sols. min_sol_ineq_sys_comm sys sols \<and> (\<forall>i. regular_lang (sols i))"
 proof -
   from eqs_reg sys_valid have
-    "\<exists>sols. partial_min_sol_ineq_sys (length sys) sys sols \<and> (\<forall>i. regular_fun (sols i))"
+    "\<exists>sols. partial_min_sol_ineq_sys (length sys) sys sols \<and> (\<forall>i. reg_eval (sols i))"
     using exists_minimal_reg_sol_sys_aux by blast
   then obtain sols where
-    sols_intro: "partial_min_sol_ineq_sys (length sys) sys sols \<and> (\<forall>i. regular_fun (sols i))"
+    sols_intro: "partial_min_sol_ineq_sys (length sys) sys sols \<and> (\<forall>i. reg_eval (sols i))"
     by blast
-  then have "const_fun (sols i)" if "i < length sys" for i
+  then have "const_rlexp (sols i)" if "i < length sys" for i
     using that unfolding partial_min_sol_ineq_sys_def by (meson equals0I leD)
   with sols_intro have "\<exists>l. regular_lang l \<and> (\<forall>v. eval (sols i) v = l)" if "i < length sys" for i
-    using that const_fun_regular_lang by metis
+    using that const_rlexp_regular_lang by metis
   then obtain ls where ls_intro: "\<forall>i < length sys. regular_lang (ls i) \<and> (\<forall>v. eval (sols i) v = ls i)"
     by metis
 
@@ -563,9 +579,9 @@ proof -
     fix sol' x
     assume as: "solves_ineq_sys_comm sys sol'"
 
-    let ?sol_funs = "\<lambda>i. Const (sol' i)"
+    let ?sol_rlexps = "\<lambda>i. Const (sol' i)"
     from as have "solves_ineq_sys_comm (take (length sys) sys) sol'" by simp
-    moreover have "sol' x = eval (?sol_funs x) sol'" for x by simp
+    moreover have "sol' x = eval (?sol_rlexps x) sol'" for x by simp
     ultimately show "\<forall>x. parikh_img (?ls' x) \<subseteq> parikh_img (sol' x)"
       using sols_intro unfolding partial_min_sol_ineq_sys_def
       by (smt (verit) empty_subsetI eval.simps(1) ls'_intro parikh_img_mono)
@@ -593,7 +609,7 @@ proof -
     with Lang_lfp_eq_Lang have ***: "Lang P S = ?sol (\<gamma>' S)" by metis
 
     from * ** CFG_eq_sys.CFL_is_min_sol obtain sys
-      where sys_intro: "(\<forall>eq \<in> set sys. regular_fun eq) \<and> (\<forall>eq \<in> set sys. \<forall>x \<in> vars eq. x < length sys)
+      where sys_intro: "(\<forall>eq \<in> set sys. reg_eval eq) \<and> (\<forall>eq \<in> set sys. \<forall>x \<in> vars eq. x < length sys)
                         \<and> min_sol_ineq_sys sys ?sol"
       unfolding CFG_eq_sys_def by blast
     with min_sol_min_sol_comm have sol_is_min_sol: "min_sol_ineq_sys_comm sys ?sol" by fast
